src/Time.v
@@ -1,0 +1,37 @@
+Require Import NArith.
+Require Import PArith.
+Require Import ZArith.
+Require Import Lia.
+Require Import EquivDec.
+Require Import sflib.
+
+Require Import Order.
+
+Set Implicit Arguments.
+
+
+Module Time.
+  Include Nat.
+
+  Definition pred_opt (ts:t): option t :=
+    match ts with
+    | O => None
+    | S n => Some n
+    end.
+
+  (* Definition le (a b:t) := a <= b. *)
+  Definition join (a b:t) := max a b.
+  Definition bot: t := 0.
+
+  Global Program Instance order: orderC join bot.
+  Next Obligation. unfold join. lia. Qed.
+  Next Obligation. unfold join. lia. Qed.
+  Next Obligation. eauto using Max.max_assoc. Qed.
+  Next Obligation. eauto using Max.max_comm. Qed.
+  Next Obligation. unfold join. lia. Qed.
+  Next Obligation. unfold bot. lia. Qed.
+
+  Global Instance eqdec: EqDec t eq := nat_eq_eqdec.
+End Time.
+
+Module View := Time.
